FullAbstractionFE.v
@@ -19,13 +19,13 @@ Require Import BacktransFE.InjectExtract.
 Require Import BacktransFE.UpgradeDowngrade.
 
 Definition backtranslateCtx n τ Cu : F.PCtx := (F.eraseAnnot_pctx (F.pctxA_cat
-                      (F.a_papp₂ τ (UValFE n (compfi_ty τ)) (injectA n τ) F.a_phole)
+                      (F.a_papp₂ τ (UValFE n (compfe_ty τ)) (injectA n τ) F.a_phole)
                       (emulate_pctx n Cu))).
 
 Lemma backtranslateCtx_works {Cu m n d p τs τu ts tu} :
   ValidTy τu →
   dir_world_prec m n d p →
-  ⟪ ea⊢ Cu : E.empty, compfi_ty τs → E.empty, τu ⟫ →
+  ⟪ ea⊢ Cu : E.empty, compfe_ty τs → E.empty, τu ⟫ →
   ⟪ pempty ⊩ ts ⟦ d, n ⟧ tu : embed τs ⟫ →
   ⟪ pempty ⊩ (F.pctx_app ts (backtranslateCtx m τs Cu)) ⟦ d, n ⟧ E.pctx_app tu (eraseAnnot_pctx
       Cu) : pEmulDV m p τu ⟫.
@@ -41,7 +41,7 @@ Lemma equivalencePreservation {t₁ t₂ τ} :
   ⟪ F.empty ⊢ t₁ : τ ⟫ →
   ⟪ F.empty ⊢ t₂ : τ ⟫ →
   ⟪ F.empty ⊢ t₁ ≃ t₂ : τ ⟫ →
-  ⟪ E.empty e⊢ compfi t₁ ≃ compfi t₂ : compfi_ty τ ⟫.
+  ⟪ E.empty e⊢ compfe t₁ ≃ compfe t₂ : compfe_ty τ ⟫.
 Proof.
   (* sufficient to prove one direction of equi-termination *)
   revert t₁ t₂ τ.
@@ -50,8 +50,8 @@ Proof.
             ⟪ F.empty ⊢ t₁ : τ ⟫ →
             ⟪ F.empty ⊢ t₂ : τ ⟫ →
             ⟪ F.empty ⊢ t₁ ≃ t₂ : τ ⟫ →
-            ∀ {C}, ⟪ ea⊢ C : E.empty , compfi_ty τ → E.empty , τ' ⟫ →
-                 E.Terminating (E.pctx_app (compfi t₁) (eraseAnnot_pctx C)) → E.Terminating (E.pctx_app (compfi t₂) (eraseAnnot_pctx C))) as Hltor
+            ∀ {C}, ⟪ ea⊢ C : E.empty , compfe_ty τ → E.empty , τ' ⟫ →
+                 E.Terminating (E.pctx_app (compfe t₁) (eraseAnnot_pctx C)) → E.Terminating (E.pctx_app (compfe t₂) (eraseAnnot_pctx C))) as Hltor
       by (intros t₁ t₂ τ ty1 ty2 ceq;
           assert (⟪ F.empty ⊢ t₂ ≃ t₁ : τ ⟫)
             by (apply F.pctx_equiv_symm; assumption);
@@ -61,9 +61,9 @@ Proof.
   intros t₁ t₂ τ τ' vτ' ty₁ ty₂ ceq Cu tCu term.
   destruct (E.Terminating_TermHor term) as [n termN]; clear term.
 
-  assert (⟪ pempty ⊩ t₁ ⟦ dir_gt , S n ⟧ compfi t₁ : embed τ ⟫) as lre₁
+  assert (⟪ pempty ⊩ t₁ ⟦ dir_gt , S n ⟧ compfe t₁ : embed τ ⟫) as lre₁
       by (change pempty with (embedCtx (repEmulCtx pempty)); 
-          eapply compfi_correct;
+          eapply compfe_correct;
           cbn; assumption).
 
   unshelve epose proof (lrfull₁ := backtranslateCtx_works vτ' (dwp_precise _) tCu lre₁).
@@ -78,11 +78,11 @@ Proof.
                                     (F.eraseAnnot_pctx (emulate_pctx (S (S n)) Cu)))) as termF
     by (eapply (adequacy_gt lrfull₁ termN); eauto with arith).
 
-  change (F.app (inject (S (S n)) τ) t₁) with (F.pctx_app t₁ (F.eraseAnnot_pctx (F.a_papp₂ τ (UValFE (S (S n)) (compfi_ty τ)) (injectA (S (S n)) τ) F.a_phole))) in termF.
+  change (F.app (inject (S (S n)) τ) t₁) with (F.pctx_app t₁ (F.eraseAnnot_pctx (F.a_papp₂ τ (UValFE (S (S n)) (compfe_ty τ)) (injectA (S (S n)) τ) F.a_phole))) in termF.
   rewrite <- F.pctx_cat_app in termF.
   rewrite <- F.eraseAnnot_pctx_cat in termF.
 
-  assert (⟪ ⊢ F.eraseAnnot_pctx (emulate_pctx (S (S n)) Cu) : F.empty, UValFE (S (S n)) (compfi_ty τ) → F.empty, UValFE (S (S n)) τ' ⟫) by
+  assert (⟪ ⊢ F.eraseAnnot_pctx (emulate_pctx (S (S n)) Cu) : F.empty, UValFE (S (S n)) (compfe_ty τ) → F.empty, UValFE (S (S n)) τ' ⟫) by
     (change F.empty with (toUVals (S (S n)) E.empty);
         eapply F.eraseAnnot_pctxT, emulate_pctx_T; eauto with tyvalid).
 
@@ -95,9 +95,9 @@ Proof.
 
   destruct (F.Terminating_TermHor termS') as [m termSm']; clear termS'.
 
-  assert (⟪ pempty ⊩ t₂ ⟦ dir_lt , S m ⟧ compfi t₂ : embed τ ⟫) as lre₂
+  assert (⟪ pempty ⊩ t₂ ⟦ dir_lt , S m ⟧ compfe t₂ : embed τ ⟫) as lre₂
       by (change pempty with (embedCtx (repEmulCtx pempty)); 
-          eapply compfi_correct;
+          eapply compfe_correct;
           cbn; assumption).
 
   epose proof (lrfull₂ := backtranslateCtx_works vτ' dwp_imprecise tCu lre₂).
@@ -108,7 +108,7 @@ Definition FullAbstraction (t₁ : F.Tm) (t₂ : F.Tm) (τ : F.Ty) : Prop :=
   ⟪ F.empty ⊢ t₁ : τ ⟫ →
   ⟪ F.empty ⊢ t₂ : τ ⟫ →
   ⟪ F.empty ⊢ t₁ ≃ t₂ : τ ⟫ ↔
-  ⟪ E.empty e⊢ compfi t₁ ≃ compfi t₂ : compfi_ty τ ⟫.
+  ⟪ E.empty e⊢ compfe t₁ ≃ compfe t₂ : compfe_ty τ ⟫.
 
 Lemma fullAbstraction {t₁ t₂ τ} : FullAbstraction t₁ t₂ τ.
 Proof.
